# State function, dealing with partial derivatives

This is a preparation for next chapter. This chapter covers some concept
required for next chapter.\

## State Function

Let $f$ be a function of $x$ and $y$

$$f(x,y)$$

Total differential

$$\begin{align*}
df &= \underset{\downarrow}{\underline{\left(\frac{\partial f}{\partial x}\right)_y}} dx + \underset{\downarrow}{\underline{\left(\frac{\partial f}{\partial y}\right)_x}} dy \\
&= M(x,y)dx + N(x,y) dy
\end{align*}$$

This expression is called \"exact\" if

$$\frac{\partial M}{\partial y} = \frac{\partial N}{\partial x}$$

$$\begin{align*}
 \frac{\partial^2 f}{\partial x \partial y} = \frac{\partial^2 f}{\partial y \partial x} & \leftarrow \begin{tabular}{l} This is always\\ true when $f"$ is continuous\\ (from Real Analysis) \end{tabular}
\end{align*}$$

Important point is that\
$$df= M(x,y)dx + N(x,y)dy \text{ is "exact" \circled{i.e.} } \frac{\partial M}{\partial y} = \frac{\partial N}{\partial x}$$

$$\Updownarrow$$

$$f(x,y)= \int_C M(x,y)dx + N(x,y)dy \text{ is path independent.}$$

:::: wrapfigure
r0.5

::: center
![image](images/cyclic.png){width="35%"}
:::
::::

This means that line integral is $\int_C df=f(x_f,y_f)-f(x_i,y_i)$. Now,
consider cyclic path($(x_1,y_1)$ to $(x_2,y_2)$ then back to
$(x_1,y_1)$). The integral on this cyclic path(regardress of path you
choose) is zero. Thermodynamically, this means that state specified by
the variable x and y is unique (state function). The concept of state
function is useful in thermodynamics and you will use this property in
Part 2 of this textbook.\

Example: Ideal Gas\
From general chemistry I, (We will derive this formula later)\
Note: gas constant R:=avogadro number$\times k_B$ $$PV = nRT$$

$$V = \frac{RT}{P} \hspace{5pt} n=1$$

$V(T,P)$

$$dV = \left(\frac{\partial V}{\partial P}\right)_TdP + \left(\frac{\partial V}{\partial T}\right)_P dT$$

$$\left(\frac{\partial V}{\partial P}\right)_T = -\frac{RT}{P^2} \hspace{10pt} \left(\frac{\partial V}{\partial T}\right)_P = \frac{R}{P}$$

So,

$$dV = -\frac{RT}{P^2}dP + \frac{R}{P}dT$$

$$\frac{\partial^2 V}{\partial T \partial P} = -\frac{R}{P^2} = \frac{\partial^2V}{\partial P \partial T}$$

So, $dV$ is exact & $\Delta V$ is path independent for the ideal gas
system. This should be intuitively obvious to us. Volume change is a
volume change no matter what path it takes.

## Useful Mathematical Relations

Math Exercise: Obtain $\left(\frac{\partial P}{\partial T}\right)_V$.\
Let

$$V = V(P,T).$$

Then,

$$dV = \left(\frac{\partial V}{\partial P}\right)_TdP + \left(\frac{\partial V}{\partial T}\right)_P dT$$

$$\begin{align*}
\left(\frac{dV}{dT}\right)_V &= \left(\frac{\partial V}{\partial P}\right)_T\left(\frac{dP}{dT}\right)_V + \left(\frac{\partial V}{\partial T}\right)_P\\
&=0 \hspace{10pt} (\because dV \text{ at } V \text{ const.})
\end{align*}$$

Then, $$\begin{align*}
\left(\frac{\partial P}{\partial T}\right)_V &= - \frac{\left(\frac{\partial V}{\partial T}\right)_P}{\left(\frac{\partial V}{\partial P}\right)_T} \\ 
& \text{and}\\
& = \frac{\frac{1}{V}\left(\frac{\partial V}{\partial T}\right)_P}{\frac{-1}{V}\left(\frac{\partial V}{\partial P}\right)_T} =\frac{\alpha}{\kappa}\cdots \text{\circled{1}}\\
\end{align*}$$

The numerator ($\alpha$) and denominator($\beta$) are called coefficient
of thermal expansion, and coefficient of compressibility, respectively.\
Obtain $\left(\frac{\partial T}{\partial P}\right)_V$.

$$dV = \left(\frac{\partial V}{\partial P}\right)_TdP + \left(\frac{\partial V}{\partial T}\right)_PdT$$

Const. V.

$$\begin{align*}
\left(\frac{\partial V}{\partial P}\right)_V &= \left(\frac{\partial V}{\partial P}\right)_T + \left(\frac{\partial V}{\partial T}\right)_P
 \left(\frac{\partial T}{\partial P}\right)_V = 0\\
 \left(\frac{\partial T}{\partial P}\right)_V &= \frac{- \left(\frac{\partial V}{\partial P}\right)_T}{ \left(\frac{\partial V}{\partial T}\right)_P} \cdots \text{\circled{2}}
\end{align*}$$

From & ,

$$\left(\frac{\partial P}{\partial T}\right)_V = \frac{1}{ \left(\frac{\partial T}{\partial P}\right)_V}$$

In general,

$$\left(\frac{\partial x}{\partial y}\right)_z = \frac{1}{ \left(\frac{\partial y}{\partial x}\right)_z} \cdots \text{ inverter }$$

Assume variation of $x$ & $y$ does not affect $z$.

($z$ indep of $x$, $y$)

$$dz =  \left(\frac{\partial z}{\partial x}\right)_y dx +  \left(\frac{\partial z}{\partial y}\right)_x dy = 0$$

const. $z$.

$$\left(\frac{\partial z}{\partial x}\right)_y \left(\frac{\partial x}{\partial y}\right)_z +  \left(\frac{\partial z}{\partial y}\right)_x = 0$$

by $\left(\frac{\partial y}{\partial z}\right)_x$,

$$\left(\frac{\partial z}{\partial x}\right)_y \left(\frac{\partial x}{\partial y}\right)_z  \left(\frac{\partial y}{\partial z}\right)_x = -1$$

[HW]{.underline}\
Show

$$\left(\frac{\partial x}{\partial z}\right)_y \left(\frac{\partial z}{\partial y}\right)_x  \left(\frac{\partial y}{\partial x}\right)_z = -1$$

Show

$$\left(\frac{\partial x}{\partial y}\right)_z = -\left(\frac{\partial z}{\partial y}\right)_x  \left(\frac{\partial x}{\partial z}\right)_y$$
